Sure, let's calculate the backpropagation for one step.

First, let's calculate the forward propagation:

1. Calculate the weighted sum for the hidden layer:
   - $z_{h1} = w_1 \cdot x_1 + w_3 \cdot x_2 + b_1 = 0.3 \cdot 0 + 0.2 \cdot 1 + 0.2 = 0.4$
   - $z_{h2} = w_2 \cdot x_1 + w_4 \cdot x_2 + b_2 = 0.2 \cdot 0 - 0.6 \cdot 1 - 1.4 = -2$

2. Apply the LreLU activation function:
   - $h_1 = LreLU(z_{h1}) = 0.4$ (since $z_{h1} \geq 0$)
   - $h_2 = LreLU(z_{h2}) = 0.2 \cdot -2 = -0.4$ (since $z_{h2} < 0$)

3. Calculate the weighted sum for the output layer:
   - $z_y = w_5 \cdot h_1 + w_6 \cdot h_2 = 0.5 \cdot 0.4 - 1 \cdot -0.4 = 0.6$

4. Apply the sigmoid activation function to get the predicted output:
   - $\hat{y} = sigmoid(z_y) = \frac{1}{1 + e^{-0.6}} \approx 0.65$

5. Calculate the loss:
   - $L = \frac{1}{2}(\hat{y} - y)^2 = \frac{1}{2}(0.65 - 1)^2 \approx 0.06$

Now, let's calculate the backpropagation:

1. Calculate the derivative of the loss with respect to the predicted output:
   - $\frac{dL}{d\hat{y}} = \hat{y} - y = 0.65 - 1 = -0.35$

2. Calculate the derivative of the predicted output with respect to the weighted sum of the output layer:
   - $\frac{d\hat{y}}{dz_y} = \hat{y} \cdot (1 - \hat{y}) = 0.65 \cdot (1 - 0.65) \approx 0.23$

3. Calculate the derivative of the weighted sum of the output layer with respect to the weights and the outputs of the hidden layer:
   - $\frac{dz_y}{dw_5} = h_1 = 0.4$
   - $\frac{dz_y}{dw_6} = h_2 = -0.4$
   - $\frac{dz_y}{dh_1} = w_5 = 0.5$
   - $\frac{dz_y}{dh_2} = w_6 = -1$

4. Calculate the derivative of the outputs of the hidden layer with respect to the weighted sum of the hidden layer:
   - $\frac{dh_1}{dz_{h1}} = 1$ (since $z_{h1} \geq 0$)
   - $\frac{dh_2}{dz_{h2}} = 0.2$ (since $z_{h2} < 0$)

5. Calculate the derivative of the weighted sum of the hidden layer with respect to the weights, biases, and inputs:
   - $\frac{dz_{h1}}{dw_1} = x_1 = 0$
   - $\frac{dz_{h1}}{dw_3} = x_2 = 1$
   - $\frac{dz_{h1}}{db_1} = 1$
   - $\frac{dz_{h2}}{dw_2} = x_1 = 0$
   - $\frac{dz_{h2}}{dw_4} = x_2 = 1$
   - $\frac{dz_{h2}}{db_2} = 1$

Finally, let's update the weights and biases using the chain rule and the learning rate ($\alpha = 0.1$):

- $w_5 = w_5 - \alpha \cdot \frac{dL}{d\hat{y}} \cdot \frac{d\hat{y}}{dz_y} \cdot \frac{dz_y}{dw_5} \approx 0.5 - 0.1 \cdot -0.35 \cdot 0.23 \cdot 0.4 \approx 0.51$
- $w_6 = w_6 - \alpha \cdot \frac{dL}{d\hat{y}} \cdot \frac{d\hat{y}}{dz_y} \cdot \frac{dz_y}{dw_6} \approx -1 - 0.1 \cdot -0.35 \cdot 0.23 \cdot -0.4 \approx -1.01$
- $w_1 = w_1 - \alpha \cdot \frac{dL}{d\hat{y}} \cdot \frac{d\hat{y}}{dz_y} \cdot \frac{dz_y}{dh_1} \cdot \frac{dh_1}{dz_{h1}} \cdot \frac{dz_{h1}}{dw_1} = 0.3$ (since $x_1 = 0$)
- $w_2 = w_2 - \alpha \cdot \frac{dL}{d\hat{y}} \cdot \frac{d\hat{y}}{dz_y} \cdot \frac{dz_y}{dh_2} \cdot \frac{dh_2}{dz_{h2}} \cdot \frac{dz_{h2}}{dw_2} = 0.2$ (since $x_1 = 0$)
- $w_3 = w_3 - \alpha \cdot \frac{dL}{d\hat{y}} \cdot \frac{d\hat{y}}{dz_y} \cdot \frac{dz_y}{dh_1} \cdot \frac{dh_1}{dz_{h1}} \cdot \frac{dz_{h1}}{dw_3} \approx 0.2 - 0.1 \cdot -0.35 \cdot 0.23 \cdot 0.5 \cdot 1 \cdot 1 \approx 0.21$
- $w_4 = w_4 - \alpha \cdot \frac{dL}{d\hat{y}} \cdot \frac{d\hat{y}}{dz_y} \cdot \frac{dz_y}{dh_2} \cdot \frac{dh_2}{dz_{h2}} \cdot \frac{dz_{h2}}{dw_4} \approx -0.6 - 0.1 \cdot -0.35 \cdot 0.23 \cdot -1 \cdot 0.2 \cdot 1 \approx -0.59$
- $b_1 = b_1 - \alpha \cdot \frac{dL}{d\hat{y}} \cdot \frac{d\hat{y}}{dz_y} \cdot \frac{dz_y}{dh_1} \cdot \frac{dh_1}{dz_{h1}} \cdot \frac{dz_{h1}}{db_1} \approx 0.2 - 0.1 \cdot -0.35 \cdot 0.23 \cdot 0.5 \cdot 1 \cdot 1 \approx 0.21$
- $b_2 = b_2 - \alpha \cdot \frac{dL}{d\hat{y}} \cdot \frac{d\hat{y}}{dz_y} \cdot \frac{dz_y}{dh_2} \cdot \frac{dh_2}{dz_{h2}} \cdot \frac{dz_{h2}}{db_2} \approx -1.4 - 0.1 \cdot -0.35 \cdot 0.23 \cdot -1 \cdot 0.2 \cdot 1 \approx -1.39$

So, the updated weights and biases are $[w_1, w_2, w_3, w_4] \approx [0.3, 0.2, 0.21, -0.59]$, $[w_5, w_6] \approx [0.51, -1.01]$, and $[b_1, b_2] \approx [0.21, -1.39]$.
